Weidenbach_Book/IsaSAT_Watch_List.thy
@@ -18,4 +18,17 @@ text \<open>There is not much to say about watch lists since they are arrays of 
   for eq.atree.braun.7.unsat.cnf instead of 7s).
 \<close>
 
+definition mop_append_ll :: "'a list list \<Rightarrow> nat literal \<Rightarrow> 'a \<Rightarrow> 'a list list nres" where
+  \<open>mop_append_ll xs i x = do {
+     ASSERT(nat_of_lit i < length xs);
+     RETURN (append_ll xs (nat_of_lit i) x)
+  }\<close>
+
+lemma mop_append_ll:
+   \<open>(uncurry2 mop_append_ll, uncurry2 (RETURN ooo (\<lambda>W i x. W(i := W i @ [x])))) \<in>
+    [\<lambda>((W, i), x). i \<in># \<L>\<^sub>a\<^sub>l\<^sub>l \<A>]\<^sub>f \<langle>Id\<rangle>map_fun_rel (D\<^sub>0 \<A>) \<times>\<^sub>f Id \<times>\<^sub>f Id \<rightarrow> \<langle>\<langle>Id\<rangle>map_fun_rel (D\<^sub>0 \<A>)\<rangle>nres_rel\<close>
+  unfolding uncurry_def mop_append_ll_def
+  by (intro frefI nres_relI)
+    (auto intro!: ASSERT_leI simp: map_fun_rel_def append_ll_def)
+
 end
