Weidenbach_Book/IsaSAT_Setup_LLVM.thy
@@ -20,29 +20,32 @@ abbreviation stats_rel :: \<open>(stats \<times> stats) set\<close> where
 
 abbreviation ema_rel :: \<open>(ema\<times>ema) set\<close> where
   \<open>ema_rel \<equiv> word64_rel \<times>\<^sub>r word64_rel \<times>\<^sub>r word64_rel \<times>\<^sub>r word64_rel \<times>\<^sub>r word64_rel\<close>
-     
+
 abbreviation ema_assn :: \<open>ema \<Rightarrow> ema \<Rightarrow> assn\<close> where
   \<open>ema_assn \<equiv> word64_assn *a word64_assn *a word64_assn *a word64_assn *a word64_assn\<close>
 
 abbreviation stats_assn :: \<open>stats \<Rightarrow> stats \<Rightarrow> assn\<close> where
   \<open>stats_assn \<equiv> word64_assn *a word64_assn *a word64_assn *a ema_assn\<close>
-  
-  
-lemma [sepref_import_param]: 
-  "(ema_get_value, ema_get_value) \<in> ema_rel \<rightarrow> word64_rel" 
+
+
+lemma [sepref_import_param]:
+  "(ema_get_value, ema_get_value) \<in> ema_rel \<rightarrow> word64_rel"
   "(ema_bitshifting,ema_bitshifting) \<in> word64_rel"
   "(ema_reinit,ema_reinit) \<in> ema_rel \<rightarrow> ema_rel"
   "(ema_init,ema_init) \<in> word_rel \<rightarrow> ema_rel"
   by auto
 
 
-lemma ema_get_value_inline[llvm_inline]: "ema_get_value = fst" by auto
-lemma ema_bitshifting_inline[llvm_inline]: "ema_bitshifting = (0x100000000::_::len word)" by (auto simp: ema_bitshifting_def)
-lemma ema_reinit_inline[llvm_inline]: "ema_reinit = (\<lambda>(value, \<alpha>, \<beta>, wait, period). (value, \<alpha>, 0x100000000::_::len word, 0::_ word, 0:: _ word))"
+lemma ema_bitshifting_inline[llvm_inline]:
+  "ema_bitshifting = (0x100000000::_::len word)" by (auto simp: ema_bitshifting_def)
+lemma ema_reinit_inline[llvm_inline]:
+  "ema_reinit = (\<lambda>(value, \<alpha>, \<beta>, wait, period).
+    (value, \<alpha>, 0x100000000::_::len word, 0::_ word, 0:: _ word))"
   by auto
+
 lemmas [llvm_inline] = ema_init_def
 
-sepref_def ema_update_impl is "uncurry (RETURN oo ema_update)"  
+sepref_def ema_update_impl is "uncurry (RETURN oo ema_update)"
   :: "uint32_nat_assn\<^sup>k *\<^sub>a ema_assn\<^sup>k \<rightarrow>\<^sub>a ema_assn"
   unfolding ema_update_def
   apply (rewrite at \<open>let _ = of_nat \<hole> * _ in _\<close> annot_unat_unat_upcast[where 'l = 64])
@@ -53,13 +56,13 @@ sepref_def ema_update_impl is "uncurry (RETURN oo ema_update)"
   by sepref
 
 lemma [sepref_import_param]:
-  "(incr_propagation,incr_propagation) \<in> stats_rel \<rightarrow> stats_rel" 
-  "(incr_conflict,incr_conflict) \<in> stats_rel \<rightarrow> stats_rel" 
-  "(incr_decision,incr_decision) \<in> stats_rel \<rightarrow> stats_rel" 
-  "(incr_restart,incr_restart) \<in> stats_rel \<rightarrow> stats_rel" 
-  "(incr_lrestart,incr_lrestart) \<in> stats_rel \<rightarrow> stats_rel" 
-  "(incr_uset,incr_uset) \<in> stats_rel \<rightarrow> stats_rel" 
-  "(incr_GC,incr_GC) \<in> stats_rel \<rightarrow> stats_rel" 
+  "(incr_propagation,incr_propagation) \<in> stats_rel \<rightarrow> stats_rel"
+  "(incr_conflict,incr_conflict) \<in> stats_rel \<rightarrow> stats_rel"
+  "(incr_decision,incr_decision) \<in> stats_rel \<rightarrow> stats_rel"
+  "(incr_restart,incr_restart) \<in> stats_rel \<rightarrow> stats_rel"
+  "(incr_lrestart,incr_lrestart) \<in> stats_rel \<rightarrow> stats_rel"
+  "(incr_uset,incr_uset) \<in> stats_rel \<rightarrow> stats_rel"
+  "(incr_GC,incr_GC) \<in> stats_rel \<rightarrow> stats_rel"
   "(add_lbd,add_lbd) \<in> word64_rel \<rightarrow> stats_rel \<rightarrow> stats_rel"
   by auto
 
@@ -72,15 +75,17 @@ lemmas [llvm_inline] =
   incr_uset_def
   incr_GC_def
 
-  
+
 abbreviation (input) "restart_info_rel \<equiv> word64_rel \<times>\<^sub>r word64_rel"
 
 abbreviation (input) restart_info_assn where
   \<open>restart_info_assn \<equiv> word64_assn *a word64_assn\<close>
 
-lemma restart_info_params[sepref_import_param]:  
-  "(incr_conflict_count_since_last_restart,incr_conflict_count_since_last_restart) \<in> restart_info_rel \<rightarrow> restart_info_rel"
-  "(restart_info_update_lvl_avg,restart_info_update_lvl_avg) \<in> word32_rel \<rightarrow> restart_info_rel \<rightarrow> restart_info_rel"
+lemma restart_info_params[sepref_import_param]:
+  "(incr_conflict_count_since_last_restart,incr_conflict_count_since_last_restart) \<in>
+    restart_info_rel \<rightarrow> restart_info_rel"
+  "(restart_info_update_lvl_avg,restart_info_update_lvl_avg) \<in>
+    word32_rel \<rightarrow> restart_info_rel \<rightarrow> restart_info_rel"
   "(restart_info_init,restart_info_init) \<in> restart_info_rel"
   "(restart_info_restart_done,restart_info_restart_done) \<in> restart_info_rel \<rightarrow> restart_info_rel"
   by auto
@@ -90,10 +95,10 @@ lemmas [llvm_inline] =
   restart_info_update_lvl_avg_def
   restart_info_init_def
   restart_info_restart_done_def
-  
-  
-(* TODO: Define vmtf_node_rel, such that sepref sees syntactically an assertion of form "pure ..."*)  
-type_synonym vmtf_node_assn = "(64 word \<times> 32 word \<times> 32 word)"    
+
+
+(* TODO: Define vmtf_node_rel, such that sepref sees syntactically an assertion of form "pure ..."*)
+type_synonym vmtf_node_assn = "(64 word \<times> 32 word \<times> 32 word)"
 
 definition "vmtf_node1_rel \<equiv> { ((a,b,c),(VMTF_Node a b c)) | a b c. True}"
 definition "vmtf_node2_assn \<equiv> uint64_nat_assn *a atom.option_assn *a atom.option_assn"
@@ -109,52 +114,60 @@ lemma vmtf_node_assn_pure[safe_constraint_rules]: \<open>CONSTRAINT is_pure vmtf
 
 (*
 
-  TODO: Test whether this setup is safe in general? 
+  TODO: Test whether this setup is safe in general?
     E.g., synthesize destructors when side-tac can prove is_pure.
-  
+
 lemmas [sepref_frame_free_rules] = mk_free_is_pure
 lemmas [simp] = vmtf_node_assn_pure[unfolded CONSTRAINT_def]
 *)
 
-lemmas [sepref_frame_free_rules] = mk_free_is_pure[OF vmtf_node_assn_pure[unfolded CONSTRAINT_def]]  
+lemmas [sepref_frame_free_rules] = mk_free_is_pure[OF vmtf_node_assn_pure[unfolded CONSTRAINT_def]]
 
 
-lemma 
+lemma
     vmtf_Node_refine1: "(\<lambda>a b c. (a,b,c), VMTF_Node) \<in> Id \<rightarrow> Id \<rightarrow> Id \<rightarrow> vmtf_node1_rel"
-and vmtf_stamp_refine1: "(\<lambda>(a,b,c). a, stamp) \<in> vmtf_node1_rel \<rightarrow> Id"  
-and vmtf_get_prev_refine1: "(\<lambda>(a,b,c). b, get_prev) \<in> vmtf_node1_rel \<rightarrow> \<langle>Id\<rangle>option_rel"  
-and vmtf_get_next_refine1: "(\<lambda>(a,b,c). c, get_next) \<in> vmtf_node1_rel \<rightarrow> \<langle>Id\<rangle>option_rel"  
+and vmtf_stamp_refine1: "(\<lambda>(a,b,c). a, stamp) \<in> vmtf_node1_rel \<rightarrow> Id"
+and vmtf_get_prev_refine1: "(\<lambda>(a,b,c). b, get_prev) \<in> vmtf_node1_rel \<rightarrow> \<langle>Id\<rangle>option_rel"
+and vmtf_get_next_refine1: "(\<lambda>(a,b,c). c, get_next) \<in> vmtf_node1_rel \<rightarrow> \<langle>Id\<rangle>option_rel"
   by (auto simp: vmtf_node1_rel_def)
 
-sepref_def VMTF_Node_impl is [] "uncurry2 (RETURN ooo (\<lambda>a b c. (a,b,c)))" :: "uint64_nat_assn\<^sup>k *\<^sub>a (atom.option_assn)\<^sup>k *\<^sub>a (atom.option_assn)\<^sup>k \<rightarrow>\<^sub>a vmtf_node2_assn"
+sepref_def VMTF_Node_impl is []
+  "uncurry2 (RETURN ooo (\<lambda>a b c. (a,b,c)))"
+  :: "uint64_nat_assn\<^sup>k *\<^sub>a (atom.option_assn)\<^sup>k *\<^sub>a (atom.option_assn)\<^sup>k \<rightarrow>\<^sub>a vmtf_node2_assn"
   unfolding vmtf_node2_assn_def by sepref
 
-sepref_def VMTF_stamp_impl is [] "RETURN o (\<lambda>(a,b,c). a)" :: "vmtf_node2_assn\<^sup>k \<rightarrow>\<^sub>a uint64_nat_assn"
-  unfolding vmtf_node2_assn_def 
+sepref_def VMTF_stamp_impl
+  is [] "RETURN o (\<lambda>(a,b,c). a)"
+  :: "vmtf_node2_assn\<^sup>k \<rightarrow>\<^sub>a uint64_nat_assn"
+  unfolding vmtf_node2_assn_def
   by sepref
 
-sepref_def VMTF_get_prev_impl is [] "RETURN o (\<lambda>(a,b,c). b)" :: "vmtf_node2_assn\<^sup>k \<rightarrow>\<^sub>a atom.option_assn"
-  unfolding vmtf_node2_assn_def 
+sepref_def VMTF_get_prev_impl
+  is [] "RETURN o (\<lambda>(a,b,c). b)"
+  :: "vmtf_node2_assn\<^sup>k \<rightarrow>\<^sub>a atom.option_assn"
+  unfolding vmtf_node2_assn_def
   by sepref
 
-sepref_def VMTF_get_next_impl is [] "RETURN o (\<lambda>(a,b,c). c)" :: "vmtf_node2_assn\<^sup>k \<rightarrow>\<^sub>a atom.option_assn"
-  unfolding vmtf_node2_assn_def 
+sepref_def VMTF_get_next_impl
+  is [] "RETURN o (\<lambda>(a,b,c). c)"
+  :: "vmtf_node2_assn\<^sup>k \<rightarrow>\<^sub>a atom.option_assn"
+  unfolding vmtf_node2_assn_def
   by sepref
 
 (* TODO: This should be done automatically! For all structured ID-relations on hr_comp! *)
 lemma workaround_hrcomp_id_norm[fcomp_norm_unfold]: "hr_comp R (\<langle>nat_rel\<rangle>option_rel) = R" by simp
 
-lemmas [sepref_fr_rules] = 
-  VMTF_Node_impl.refine[FCOMP vmtf_Node_refine1]  
+lemmas [sepref_fr_rules] =
+  VMTF_Node_impl.refine[FCOMP vmtf_Node_refine1]
   VMTF_stamp_impl.refine[FCOMP vmtf_stamp_refine1]
   VMTF_get_prev_impl.refine[FCOMP vmtf_get_prev_refine1]
   VMTF_get_next_impl.refine[FCOMP vmtf_get_next_refine1]
-  
 
-  
-    
-type_synonym vmtf_assn = \<open>vmtf_node_assn ptr \<times> 64 word \<times> 32 word \<times> 32 word \<times> 32 word\<close>  
-  
+
+
+
+type_synonym vmtf_assn = \<open>vmtf_node_assn ptr \<times> 64 word \<times> 32 word \<times> 32 word \<times> 32 word\<close>
+
 type_synonym vmtf_remove_assn = \<open>vmtf_assn \<times> (32 word array_list64 \<times> 1 word ptr)\<close>
 
 
@@ -186,21 +199,19 @@ where
 lemma workaround_opt_assn: "RETURN o (\<lambda>(a,b,c). f a b c) = (\<lambda>(a,b,c). RETURN (f a b c))" by auto
 
 sepref_register opts_restart opts_reduce opts_unbounded_mode
-  
-sepref_def opts_restart_impl is "RETURN o opts_restart" :: "opts_assn\<^sup>k \<rightarrow>\<^sub>a bool1_assn"  
+
+sepref_def opts_restart_impl is "RETURN o opts_restart" :: "opts_assn\<^sup>k \<rightarrow>\<^sub>a bool1_assn"
   unfolding opts_restart_def workaround_opt_assn opts_assn_def
   by sepref
 
-sepref_def opts_reduce_impl is "RETURN o opts_reduce" :: "opts_assn\<^sup>k \<rightarrow>\<^sub>a bool1_assn"  
+sepref_def opts_reduce_impl is "RETURN o opts_reduce" :: "opts_assn\<^sup>k \<rightarrow>\<^sub>a bool1_assn"
   unfolding opts_reduce_def workaround_opt_assn opts_assn_def
   by sepref
 
-sepref_def opts_unbounded_mode_impl is "RETURN o opts_unbounded_mode" :: "opts_assn\<^sup>k \<rightarrow>\<^sub>a bool1_assn"  
+sepref_def opts_unbounded_mode_impl is "RETURN o opts_unbounded_mode" :: "opts_assn\<^sup>k \<rightarrow>\<^sub>a bool1_assn"
   unfolding opts_unbounded_mode_def workaround_opt_assn opts_assn_def
   by sepref
-  
-  
-  
+
 abbreviation "watchlist_fast_assn \<equiv> aal_assn' TYPE(64) TYPE(64) watcher_fast_assn"
 
 
@@ -214,13 +225,14 @@ abbreviation phase_saver_assn where
 
 (* TODO: Move *)
 type_synonym arena_assn = "(32 word, 64) array_list"
-  
+
 typ "(32 word, 64) array_list"
-  
+
 type_synonym twl_st_wll_trail_fast =
   \<open>trail_pol_fast_assn \<times> arena_assn \<times> option_lookup_clause_assn \<times>
     64 word \<times> watched_wl_uint32 \<times> vmtf_remove_assn \<times> phase_saver_assn \<times>
-    32 word \<times> cach_refinement_l_assn \<times> lbd_assn \<times> out_learned_assn \<times> stats \<times> (ema \<times> ema \<times> restart_info) \<times>
+    32 word \<times> cach_refinement_l_assn \<times> lbd_assn \<times> out_learned_assn \<times> stats \<times>
+    (ema \<times> ema \<times> restart_info) \<times>
     vdom_fast_assn \<times> vdom_fast_assn \<times> 64 word \<times> opts_assn \<times> arena_assn\<close>
 
 definition heuristic_assn where
@@ -311,14 +323,14 @@ sepref_def access_lit_in_clauses_heur_fast_code
 sepref_register \<open>(=) :: clause_status \<Rightarrow> clause_status \<Rightarrow> _\<close>
 
 
-lemma [def_pat_rules]: "append_ll \<equiv> op_list_list_push_back" 
+lemma [def_pat_rules]: "append_ll \<equiv> op_list_list_push_back"
   by (rule eq_reflection) (auto simp: append_ll_def fun_eq_iff)
 
 sepref_register rewatch_heur mop_append_ll mop_arena_length
 
 sepref_def mop_append_ll_impl
   is \<open>uncurry2 mop_append_ll\<close>
-  :: \<open>[\<lambda>((W, i), _). length (W ! (nat_of_lit i)) < sint64_max]\<^sub>a 
+  :: \<open>[\<lambda>((W, i), _). length (W ! (nat_of_lit i)) < sint64_max]\<^sub>a
     watchlist_fast_assn\<^sup>d *\<^sub>a unat_lit_assn\<^sup>k *\<^sub>a watcher_fast_assn\<^sup>k \<rightarrow> watchlist_fast_assn\<close>
   unfolding mop_append_ll_def
   by sepref
@@ -326,7 +338,8 @@ sepref_def mop_append_ll_impl
 
 sepref_def rewatch_heur_fast_code
   is \<open>uncurry2 (rewatch_heur)\<close>
-  :: \<open>[\<lambda>((vdom, arena), W). (\<forall>x \<in> set vdom. x \<le> sint64_max) \<and> length arena \<le> sint64_max \<and> length vdom \<le> sint64_max]\<^sub>a
+  :: \<open>[\<lambda>((vdom, arena), W). (\<forall>x \<in> set vdom. x \<le> sint64_max) \<and> length arena \<le> sint64_max \<and>
+        length vdom \<le> sint64_max]\<^sub>a
         vdom_fast_assn\<^sup>k *\<^sub>a arena_fast_assn\<^sup>k *\<^sub>a watchlist_fast_assn\<^sup>d \<rightarrow> watchlist_fast_assn\<close>
   supply [[goals_limit=1]]
      arena_lit_pre_le_sint64_max[dest] arena_is_valid_clause_idx_le_uint64_max[dest]
@@ -336,7 +349,7 @@ sepref_def rewatch_heur_fast_code
   unfolding while_eq_nfoldli[symmetric]
   apply (subst while_upt_while_direct, simp)
   unfolding if_not_swap
-    FOREACH_cond_def FOREACH_body_def 
+    FOREACH_cond_def FOREACH_body_def
   apply (annot_snat_const "TYPE(64)")
   by sepref
 
@@ -384,7 +397,8 @@ sepref_register clause_lbd_heur
 
 
 lemma clause_lbd_heur_alt_def:
-  \<open>clause_lbd_heur = (\<lambda>(M', N', D', j, W', vm, \<phi>, clvls, cach, lbd, outl, stats, heur, vdom, lcount) C.
+  \<open>clause_lbd_heur = (\<lambda>(M', N', D', j, W', vm, \<phi>, clvls, cach, lbd, outl, stats, heur, vdom,
+     lcount) C.
      arena_lbd N' C)\<close>
   by (intro ext) (auto simp: clause_lbd_heur_def)
 
@@ -549,12 +563,12 @@ sepref_def get_pos_of_level_in_trail_imp_st_code
 
 
 
-sepref_register neq : "(op_neq :: clause_status \<Rightarrow> _ \<Rightarrow> _)" 
+sepref_register neq : "(op_neq :: clause_status \<Rightarrow> _ \<Rightarrow> _)"
 lemma status_neq_refine1: "((\<noteq>),op_neq) \<in> status_rel \<rightarrow> status_rel \<rightarrow> bool_rel"
   by (auto simp: status_rel_def)
 
-sepref_def status_neq_impl is [] "uncurry (RETURN oo (\<noteq>))" 
-  :: "(unat_assn' TYPE(32))\<^sup>k *\<^sub>a (unat_assn' TYPE(32))\<^sup>k \<rightarrow>\<^sub>a bool1_assn"  
+sepref_def status_neq_impl is [] "uncurry (RETURN oo (\<noteq>))"
+  :: "(unat_assn' TYPE(32))\<^sup>k *\<^sub>a (unat_assn' TYPE(32))\<^sup>k \<rightarrow>\<^sub>a bool1_assn"
   by sepref
 
 lemmas [sepref_fr_rules] = status_neq_impl.refine[FCOMP status_neq_refine1]
@@ -570,6 +584,73 @@ sepref_def clause_not_marked_to_delete_heur_fast_code
   supply [[goals_limit=1]]
   unfolding clause_not_marked_to_delete_heur_alt_def isasat_bounded_assn_def
      clause_not_marked_to_delete_heur_pre_def
+  by sepref
+
+lemma mop_clause_not_marked_to_delete_heur_alt_def:
+  \<open>mop_clause_not_marked_to_delete_heur = (\<lambda>(M, arena, D, oth) C. do {
+    ASSERT(clause_not_marked_to_delete_heur_pre ((M, arena, D, oth), C));
+     RETURN (arena_status arena C \<noteq> DELETED)
+   })\<close>
+  unfolding clause_not_marked_to_delete_heur_def mop_clause_not_marked_to_delete_heur_def
+  by (auto intro!: ext)
+
+sepref_def mop_clause_not_marked_to_delete_heur_impl
+  is \<open>uncurry mop_clause_not_marked_to_delete_heur\<close>
+  :: \<open>isasat_bounded_assn\<^sup>k *\<^sub>a sint64_nat_assn\<^sup>k \<rightarrow>\<^sub>a bool1_assn\<close>
+  unfolding mop_clause_not_marked_to_delete_heur_alt_def
+    clause_not_marked_to_delete_heur_pre_def  prod.case isasat_bounded_assn_def
+  by sepref
+
+sepref_def delete_index_and_swap_code2
+  is \<open>uncurry (RETURN oo delete_index_and_swap)\<close>
+  :: \<open>[\<lambda>(xs, i). i < length xs]\<^sub>a
+      vdom_fast_assn\<^sup>d *\<^sub>a sint64_nat_assn\<^sup>k \<rightarrow> vdom_fast_assn\<close>
+  unfolding delete_index_and_swap.simps
+  by sepref
+
+sepref_def mop_mark_garbage_heur_impj
+  is \<open>uncurry2 mop_mark_garbage_heur\<close>
+  :: \<open>[\<lambda>((C, i), S). length (get_clauses_wl_heur S) \<le> sint64_max]\<^sub>a
+      sint64_nat_assn\<^sup>k *\<^sub>a sint64_nat_assn\<^sup>k *\<^sub>a isasat_bounded_assn\<^sup>d \<rightarrow> isasat_bounded_assn\<close>
+  supply [[goals_limit=1]]
+  unfolding mop_mark_garbage_heur_alt_def
+    clause_not_marked_to_delete_heur_pre_def prod.case isasat_bounded_assn_def
+  apply (annot_unat_const "TYPE(64)")
+  by sepref
+
+sepref_def mop_mark_unused_st_heur_impl
+  is \<open>uncurry mop_mark_unused_st_heur\<close>
+  :: \<open> sint64_nat_assn\<^sup>k *\<^sub>a isasat_bounded_assn\<^sup>d \<rightarrow>\<^sub>a isasat_bounded_assn\<close>
+  unfolding mop_mark_unused_st_heur_def
+  by sepref
+
+
+sepref_def mop_arena_lbd_st_impl
+  is \<open>uncurry mop_arena_lbd_st\<close>
+  :: \<open>isasat_bounded_assn\<^sup>k *\<^sub>a sint64_nat_assn\<^sup>k \<rightarrow>\<^sub>a uint32_nat_assn\<close>
+  supply [[goals_limit=1]]
+  unfolding mop_arena_lbd_st_alt_def isasat_bounded_assn_def
+  by sepref
+
+sepref_def mop_arena_status_st_impl
+  is \<open>uncurry mop_arena_status_st\<close>
+  :: \<open>isasat_bounded_assn\<^sup>k *\<^sub>a sint64_nat_assn\<^sup>k \<rightarrow>\<^sub>a status_impl_assn\<close>
+  supply [[goals_limit=1]]
+  unfolding mop_arena_status_st_alt_def isasat_bounded_assn_def
+  by sepref
+
+sepref_def mop_marked_as_used_st_impl
+  is \<open>uncurry mop_marked_as_used_st\<close>
+  :: \<open>isasat_bounded_assn\<^sup>k *\<^sub>a sint64_nat_assn\<^sup>k \<rightarrow>\<^sub>a bool1_assn\<close>
+  supply [[goals_limit=1]]
+  unfolding mop_marked_as_used_st_alt_def isasat_bounded_assn_def
+  by sepref
+
+sepref_def mop_arena_length_st_impl
+  is \<open>uncurry mop_arena_length_st\<close>
+  :: \<open>isasat_bounded_assn\<^sup>k *\<^sub>a sint64_nat_assn\<^sup>k \<rightarrow>\<^sub>a sint64_nat_assn\<close>
+  supply [[goals_limit=1]]
+  unfolding mop_arena_length_st_alt_def isasat_bounded_assn_def
   by sepref
 
 
@@ -595,3 +676,4 @@ export_llvm
 end
 
 end
+
